21 sep

coq/FreeGroup.v
@@ -1,6 +1,7 @@
 Require Import Coq.Program.Equality.
 Require Import Coq.Bool.Bool.
 Require Import Coq.Lists.List.
+Require Import StrictProp.
 Import ListNotations.
 
 Class Group (A : Type) := GroupDef {
@@ -16,28 +17,35 @@ Class Group (A : Type) := GroupDef {
   eqf_eq    : forall x y, reflect (x = y) (eqf x y)
 }.
 
-Print reflect.
-
 Lemma eqf_refl {A: Type} `{Group A} (x : A) : eqf x x = true.
 Proof.
   destruct (eqf_eq x x); auto.
 Qed.
 
-Definition eqf_false {A: Type} `{Group A} {x y: A} : eqf x y = false -> x <> y.
+Definition eqf_false_iff {A: Type} `{Group A} {x y: A} : eqf x y = false <-> x <> y.
 Proof.
-  intros H0 H1. subst. rewrite eqf_refl in H0. discriminate.
+  split.
+  - intros H0 H1. subst. rewrite eqf_refl in H0. discriminate.
+  - intros H0. destruct (eqf_eq x y); auto. subst. contradiction.
 Defined.
 
-Notation "a @ b" := (op a b) (at level 50).
-Notation "c ^" := (inv c) (at level 40).
+(* Notation "a @ b" := (op a b) (at level 51, right associativity).
+Notation "c ^" := (inv c) (at level 40). *)
 
 Definition sub {A: Type} `{Group A} (x y: A) := op x (inv y).
 
 Definition CanonFreeGroup (A: Type) `{Group A} := list (bool*A).
 
+Inductive Normalized {A: Type} `{Group A} : CanonFreeGroup A -> Prop :=
+| NNil   : Normalized []
+| NSingl : forall (b : bool) (v : A), Normalized [(b, v)]
+| NCons  : forall (b b': bool) (v v' : A) (x: CanonFreeGroup A), 
+            v <> v' \/ b = b' -> Normalized ((b', v') :: x) ->
+            Normalized ((b, v) :: (b', v') :: x).
+
 Inductive NonEmptyFreeGroup (A: Type) `{Group A} :=
 | Singl  : bool -> A -> NonEmptyFreeGroup A
-| Switch : forall x: A, eqf zero x = false -> NonEmptyFreeGroup A -> NonEmptyFreeGroup A
+| Switch : forall x: A, Squash (x <> zero) -> NonEmptyFreeGroup A -> NonEmptyFreeGroup A
 | Stay   : A -> NonEmptyFreeGroup A -> NonEmptyFreeGroup A.
 
 Arguments Switch {A H}.
@@ -46,15 +54,17 @@ Arguments Singl {A H}.
 
 Definition FreeGroup (A: Type) `{Group A} := option (NonEmptyFreeGroup A).
 
+Print reflect.
+
 Fixpoint to_uniq' {A: Type} `{Group A} (b : bool) (v: A) (x: CanonFreeGroup A) : NonEmptyFreeGroup A :=
 match x with 
 | []             => Singl b v
 | (b', v') :: x' => if eqb b b' 
                       then Stay (sub v v') (to_uniq' b' v' x')
-                      else match eqf zero (sub v v') as i return (eqf zero (sub v v') = i) -> NonEmptyFreeGroup A with
-                           | false => fun e => Switch (sub v v') e (to_uniq' b' v' x')
-                           | true  => fun _ => (Singl b v) (* invalid *)
-                           end eq_refl
+                      else match eqf_eq (sub v v') zero with
+                           | ReflectF _ p => Switch (sub v v') (squash p) (to_uniq' b' v' x')
+                           | _  => (Singl b v) (* invalid *)
+                           end
 end.
 
 Definition to_uniq {A: Type} `{Group A} (x: CanonFreeGroup A) : FreeGroup A :=
@@ -65,15 +75,15 @@ end.
 
 Fixpoint to_canon' {A: Type} `{Group A} (x: NonEmptyFreeGroup A) : CanonFreeGroup A :=
   match x with 
-  | Singl b v   => [(b, v)]
-  | Stay v x'   => match to_canon' x' with
-                   | [] => [(true, v)] (* should not be there *)
-                   | (b, v') :: y => (b, (v @ v')) :: (b, v') :: y
-                   end
+  | Singl b v     => [(b, v)]
+  | Stay v x'     => match to_canon' x' with
+                     | [] => [(true, v)] (* should not be there *)
+                     | (b, v') :: y => (b, op v v') :: (b, v') :: y
+                     end
   | Switch v _ x' => match to_canon' x' with
-                               | [] => [(true, v)] (* should not be there *)
-                               | (b, v') :: y => (negb b, (v @ v')) :: (b, v') :: y
-                               end
+                     | [] => [(true, v)] (* should not be there *)
+                     | (b, v') :: y => (negb b, op v v') :: (b, v') :: y
+                     end
   end.
 
 Definition to_canon {A: Type} `{Group A} (x: FreeGroup A) : CanonFreeGroup A :=
@@ -92,17 +102,393 @@ Proof.
   unfold sub. rewrite op_assoc. rewrite right_inv. rewrite right_id. auto.
 Qed.
 
-Print reflect.
+Lemma squash_not_refl {A : Type} (x: A) (P: Prop) : Squash (x <> x) -> P.
+Proof.
+  intros H. apply sEmpty_ind. apply (Squash_sind (x <> x)); auto.
+  intro H0. exfalso. apply H0. auto.
+Qed.
 
-Theorem free_group_epi_cannon {A: Type} `{Group A} (x: FreeGroup A) : 
+Lemma not_eqb_is_neg (x y : bool) : eqb x y = false -> x = negb y.
+Proof.
+  intros H. destruct x, y; cbn in *; auto; try inversion H.
+Qed.
+
+Lemma some_eq {A: Type} (x y: A) : Some x = Some y -> x = y.
+Proof.
+  intros H. inversion H. auto.
+Qed.
+
+Lemma eqb_not_neg (x y : bool) : eqb x (negb y) = false <-> x = y.
+Proof.
+  split.
+  - intros H. destruct x, y; auto; try inversion H.
+  - intros H. subst. destruct y; auto.
+Qed.
+
+Lemma group_equation_l_simp {A: Type} `{Group A} (a b c : A) : op a b = op a c -> b = c.
+Proof.
+  intro H0. assert (op (inv a) (op a b) = op (inv a) (op a c)).
+  - rewrite H0. auto.
+  - rewrite <- op_assoc, <- op_assoc, left_inv, left_id, left_id in H1. auto.
+Qed.
+
+Lemma group_equation_r_simp {A: Type} `{Group A} (a b c : A) : op a c = op b c -> a = b.
+Proof.
+  intro H0. assert (op (op a c) (inv c) = op (op b c) (inv c)).
+  - rewrite H0. auto.
+  - rewrite op_assoc, op_assoc, right_inv, right_id, right_id in H1. auto.
+Qed.
+
+Lemma sub_inv_uniq {A: Type} `{Group A} (x y: A) : sub x y = zero -> x = y.
+Proof.
+  unfold sub. rewrite <- (right_inv y). intros H0. 
+  apply group_equation_r_simp with (c := inv y). auto.
+Qed.
+
+Theorem free_group_epi_canon {A: Type} `{Group A} (x: FreeGroup A) : 
   to_uniq (to_canon x) = x.
 Proof.
+  destruct x as [x |]; auto. induction x; auto.
+  - cbn in *. destruct (to_canon' x0); inversion IHx. destruct p. cbn in *. 
+    inversion IHx. subst. rewrite eqb_negb1, sub_op. destruct (eqf_eq x zero); auto.
+    subst. apply (squash_not_refl zero); auto.
+  - cbn in *. destruct (to_canon' x); inversion IHx. destruct p. cbn in *.
+    inversion IHx. subst. rewrite eqb_reflx, sub_op. auto.
+Qed.
+
+Theorem canon_epi_free_group {A: Type} `{Group A} (x: CanonFreeGroup A) : 
+  Normalized x -> to_canon (to_uniq x) = x.
+Proof.
+  intros N. induction N; auto. cbn in *. destruct H0 as [v_neq | b_neq].
+  - destruct (eqb b b') eqn:b_eq.
+    + cbn. rewrite IHN, op_sub. f_equal. f_equal. symmetry. apply eqb_prop. auto.
+    + destruct (eqf_eq (sub v v') zero).
+      * assert (v = v') by (apply sub_inv_uniq; auto). contradiction.
+      * cbn. rewrite IHN, op_sub. f_equal. f_equal. symmetry. apply not_eqb_is_neg. auto.
+  - subst. rewrite eqb_reflx. cbn. rewrite IHN, op_sub. auto.
+Qed.
+
+Lemma to_canon'_not_nil {A: Type} `{Group A} (x: NonEmptyFreeGroup A) : to_canon' x <> nil.
+Proof.
+  intros H0. destruct x; cbn in *.
+  - inversion H0.
+  - destruct (to_canon' x0).
+    + inversion H0.
+    + destruct p. inversion H0.
+  - destruct (to_canon' x).
+    + inversion H0.
+    + destruct p. inversion H0.
+Qed.
+
+Lemma group_add_non_zero {A: Type} `{Group A} (x y : A) : x <> zero -> op x y <> y.
+Proof.
+  intros H0 H1. apply H0. apply group_equation_r_simp with (c := op y (inv y)).
+  rewrite <- op_assoc, H1, right_inv, left_id. auto.
+Qed.
+
+Lemma group_squash_non_zero {A: Type} `{Group A} (x : A) : Squash (x <> zero) -> x <> zero.
+Proof.
+  intros H0. destruct (eqf_eq x zero); auto. subst. apply (squash_not_refl zero). auto.
+Qed. 
+
+Theorem free_group_is_normal {A: Type} `{Group A} (x: FreeGroup A) : Normalized (to_canon x).
+Proof.
   destruct x as [x |].
-  - induction x; auto.
-    + cbn in *. destruct x0.
-      * cbn. f_equal. rewrite eqb_negb1, sub_op. dependent destruction x1.
+  - induction x.
+    + cbn. constructor.
+    + dependent destruction IHx.
+      * assert (to_canon (Some x0) <> []) by (apply to_canon'_not_nil). rewrite x in H0.
+        contradiction.
+      * cbn in *. rewrite <- x. constructor; constructor. apply group_add_non_zero. 
+        apply group_squash_non_zero. auto.
+      * cbn in *. rewrite <- x. constructor.
+        -- left. apply group_add_non_zero. apply group_squash_non_zero. auto.
+        -- constructor; auto.
+    + dependent destruction IHx.
+      * assert (to_canon (Some x0) <> []) by (apply to_canon'_not_nil). rewrite x in H0.
+        contradiction.
+      * cbn in *. rewrite <- x. constructor; try right; constructor.
+      * cbn in *. rewrite <- x. constructor; try right; constructor; auto.
+  - cbn. constructor.
+Qed.
+
+Definition option_bind {A B: Type} (x: option A) (f: A -> option B) : option B :=
+  match x with
+  | None => None
+  | Some x' => f x'
+  end. 
+
+Fixpoint fg_hd' {A: Type} `{Group A} (x: NonEmptyFreeGroup A) : bool * A :=
+  match x with 
+  | Singl b v => (b, v)
+  | Stay v x' => let (b', v') := fg_hd' x' in (b', op v v')
+  | Switch v _ x' => let (b', v') := fg_hd' x' in (negb b', op v v')
+  end.
+
+Definition fg_hd {A: Type} `{Group A} (x: FreeGroup A) : option (bool * A) :=
+  option_map fg_hd' x.
+
+Theorem fg_hd_for_canon {A: Type} `{Group A} (x: CanonFreeGroup A) :
+  Normalized x -> hd_error x = fg_hd (to_uniq x).
+Proof.
+  intros H0. induction H0; auto. cbn in *. f_equal. inversion IHNormalized. destruct H0.
+  - destruct (eqb b b') eqn:e.
+    + cbn. rewrite <- H3, op_sub. rewrite eqb_true_iff in e. f_equal; auto.
+    + destruct (eqf_eq (sub v v') zero); auto. cbn. rewrite <- H3, op_sub. f_equal.
+      apply not_eqb_is_neg. auto.
+  - subst. rewrite eqb_reflx. cbn. rewrite <- H3, op_sub. auto.
+Qed.
+
+Definition fq_tail' {A: Type} `{Group A} (x: NonEmptyFreeGroup A) : FreeGroup A :=
+  match x with 
+  | Singl _ _     => None
+  | Stay _ x'     => Some x'
+  | Switch _ _ x' => Some x'
+  end.
+
+Definition fg_tail {A: Type} `{Group A} (x: FreeGroup A) : FreeGroup A :=
+  option_bind x fq_tail'.
+
+Definition fg_cons' {A: Type} `{Group A} (b: bool) (v: A) (x: NonEmptyFreeGroup A) : 
+   FreeGroup A :=
+    let (b', v') := fg_hd' x in 
+      if eqb b b'
+      then Some (Stay (sub v v') x)
+      else match eqf_eq (sub v v') zero with
+           | ReflectT _ _ => fq_tail' x
+           | ReflectF _ p => Some (Switch (sub v v') (squash p) x)
+           end.
+
+Definition fg_cons'2 {A: Type} `{Group A} (p : bool * A) (x: NonEmptyFreeGroup A) :=
+  let (b, v) := p in fg_cons' b v x.
+
+Definition fg_cons {A: Type} `{Group A} (b: bool) (v: A) (x: FreeGroup A) : FreeGroup A :=
+  match x with
+  | None => Some (Singl b v)
+  | Some x' => fg_cons' b v x'
+  end.
+
+Definition fg_cons2 {A: Type} `{Group A} (p: bool * A) (x: FreeGroup A) : FreeGroup A := 
+  let (b, v) := p in fg_cons b v x.
+ 
+Definition elem_inv {A: Type} (x : bool * A) := let (b, v) := x in (negb b, v).
+
+Theorem inv_elem_cons_is_tail {A: Type} `{Group A} (x: NonEmptyFreeGroup A) :
+  fg_cons'2 (elem_inv (fg_hd' x)) x = fq_tail' x.
+Proof.
+  destruct (fg_hd' x) eqn:hd. destruct x; cbn.
+  - inversion hd. unfold sub. rewrite eqb_negb1, right_inv.
+    destruct (eqf_eq zero zero); auto. contradiction.
+  - unfold fg_cons', sub. rewrite hd, eqb_negb1, right_inv. 
+    destruct (eqf_eq zero zero); auto. contradiction.
+  - unfold fg_cons', sub. rewrite hd, eqb_negb1, right_inv. 
+    destruct (eqf_eq zero zero); auto. contradiction.
+Qed.
+
+Definition canon_cons {A: Type} `{Group A} (b: bool) (v: A) (x: CanonFreeGroup A) :
+  CanonFreeGroup A :=
+  match x with
+  | [] => [(b, v)]
+  | (b', v') :: t => if negb (eqf v v') || eqb b b'
+                     then (b, v) :: (b', v') :: t
+                     else t
+  end.
+
+Fixpoint canon_concat {A: Type} `{Group A} (x y: CanonFreeGroup A) : CanonFreeGroup A :=
+  match x with
+  | []           => y
+  | (b, v) :: x' => canon_cons b v (canon_concat x' y)
+  end.
+
+Definition fg_canon_concat {A: Type} `{Group A} (x y: FreeGroup A) : FreeGroup A :=
+  to_uniq (canon_concat (to_canon x) (to_canon y)).
+
+Theorem concat_norm {A: Type} `{Group A} (x y: CanonFreeGroup A) : 
+  Normalized x -> Normalized y -> Normalized (canon_concat x y).
+Proof.
+  intros Nx Ny. induction Nx; auto.
+  - cbn. destruct Ny; unfold canon_cons.
+    + constructor.
+    + destruct (negb (eqf v v0) || eqb b b0 ) eqn:e; constructor.
+      * rewrite orb_true_iff, eqb_true_iff, negb_true_iff, eqf_false_iff in e. auto.
+      * constructor.
+    + destruct (negb (eqf v v0) || eqb b b0) eqn:e; auto. constructor.
+      * rewrite orb_true_iff, eqb_true_iff, negb_true_iff, eqf_false_iff in e. auto.
+      * constructor; auto.
+  - cbn. destruct (canon_concat x y) eqn:c; unfold canon_cons in *.
+    + assert (negb (eqf v v') || eqb b b' = true).
+      * rewrite orb_true_iff, eqb_true_iff, negb_true_iff, eqf_false_iff. auto.
+      * rewrite H1. constructor; auto. constructor.
+    + destruct p. cbn in *. rewrite c in IHNx. destruct (negb (eqf v' a) || eqb b' b0) eqn:e.
+      * assert (negb (eqf v v') || eqb b b' = true); unfold canon_cons in *.
+        -- rewrite orb_true_iff, eqb_true_iff, negb_true_iff, eqf_false_iff. auto.
+        -- rewrite H1. rewrite e in IHNx. constructor; auto.
+      * cbn in *. destruct c0; try constructor. destruct p.
+        destruct (negb (eqf v a0) || eqb b b1) eqn:e1; unfold canon_cons in *; rewrite e in IHNx.
+        -- constructor; auto.
+           rewrite orb_true_iff, eqb_true_iff, negb_true_iff, eqf_false_iff in e1. auto.
+        -- dependent destruction IHNx; auto. constructor.
+Qed.
+
+Fixpoint fg_concat' {A: Type} `{Group A} (x: NonEmptyFreeGroup A) 
+  (y: FreeGroup A) : FreeGroup A :=
+  match x with
+  | Singl b v     => fg_cons b v y
+  | Stay _ x'     => fg_cons2 (fg_hd' x) (fg_concat' x' y)
+  | Switch _ _ x' => fg_cons2 (fg_hd' x) (fg_concat' x' y)
+  end.
+
+Definition fg_concat {A: Type} `{Group A} (x y: FreeGroup A) : FreeGroup A :=
+  match x with
+  | None => y
+  | Some x' => fg_concat' x' y
+  end.
+
+Lemma eqf_sub_not_zero {A: Type} `{Group A} (x y: A) : sub x y <> zero <-> eqf x y = false.
+Proof.
+  unfold sub. split.
+  - intros H0. destruct (eqf_eq x y); auto. subst. rewrite right_inv in H0. 
+    contradiction.
+  - intros H0 H1. assert (x = y) by (apply sub_inv_uniq; auto). subst.
+    rewrite eqf_refl in H0. discriminate.
+Qed.
+
+Theorem free_canon_hd'_izo {A: Type} `{Group A} (x: NonEmptyFreeGroup A) :
+  Some (fg_hd' x) = hd_error (to_canon (Some x)).
+Proof.
+  induction x; auto.
+  - cbn in *. destruct (to_canon' x0) eqn:e.
+    + exfalso. apply (to_canon'_not_nil x0). auto.
+    + destruct p. cbn in *. inversion IHx. rewrite H1. auto.
+  - cbn in *. destruct (to_canon' x) eqn:e.
+    + exfalso. apply (to_canon'_not_nil x). auto.
+    + destruct p. cbn in *. inversion IHx. rewrite H1. auto.
+Qed.
+
+Theorem free_canon_hd_izo {A: Type} `{Group A} (x: FreeGroup A) :
+  fg_hd x = hd_error (to_canon x).
+Proof.
+  destruct x as [x |]; auto. cbn. apply free_canon_hd'_izo.
+Qed.
+
+Theorem free_canon_cons_izo {A: Type} `{Group A} (b: bool) (v: A) (x: FreeGroup A) :
+  to_canon (fg_cons b v x) = canon_cons b v (to_canon x).
+Proof.
+  destruct x as [x |]; auto. unfold canon_cons. destruct x.
+  - cbn. destruct (eqb b b0) eqn:e.
+    + cbn. rewrite orb_true_r, op_sub. rewrite eqb_true_iff in e. subst. auto.
+    + destruct (eqf_eq (sub v a) zero).
+      * assert (v = a) by (apply sub_inv_uniq; auto). subst.
+        rewrite eqf_refl. cbn. auto.
+      * cbn. rewrite eqf_sub_not_zero in n. rewrite n, op_sub. cbn.
+        assert (negb b0 = b) by (symmetry; apply not_eqb_is_neg; auto). 
+        subst. auto.
+  - cbn. destruct (to_canon' x0) eqn:c.
+    + exfalso. apply (to_canon'_not_nil x0). auto.
+    + destruct p. unfold fg_cons'. cbn. assert (hd_eq : fg_hd' x0 = (b0, a)).
+      { apply some_eq. rewrite free_canon_hd'_izo. cbn. rewrite c. auto. }
+      rewrite hd_eq. destruct (eqb b (negb b0)) eqn:eb.
+      * cbn. rewrite orb_true_r, c, op_sub. rewrite eqb_true_iff in eb. subst.
+        auto.
+      * destruct (eqf_eq (sub v (op x a))).
+        -- assert (v = (op x a)) by (apply sub_inv_uniq; auto). subst.
+          rewrite eqf_refl. cbn. auto.
+        -- cbn. rewrite eqf_sub_not_zero in n. rewrite n, c. unfold sub. cbn.
+           rewrite (op_assoc  v (inv (op x a))), left_inv, right_id, negb_involutive.
+           f_equal. rewrite eqb_not_neg in eb. subst. auto.
+  - cbn. destruct (to_canon' x) eqn:c.
+    + exfalso. apply (to_canon'_not_nil x). auto.
+    + destruct p. unfold fg_cons'. cbn. assert (hd_eq : fg_hd' x = (b0, a0)).
+      { apply some_eq. rewrite free_canon_hd'_izo. cbn. rewrite c. auto. }
+      rewrite hd_eq. destruct (eqb b b0) eqn:eb.
+      * cbn. rewrite orb_true_r, c, op_sub. rewrite eqb_true_iff in eb. subst.
+        auto.
+      * destruct (eqf_eq (sub v (op a a0))).
+        -- assert (v = (op a a0)) by (apply sub_inv_uniq; auto). subst.
+          rewrite eqf_refl. cbn. auto.
+        -- cbn. rewrite eqf_sub_not_zero in n. rewrite n, c. unfold sub. cbn.
+           rewrite (op_assoc  v (inv (op a a0))), left_inv, right_id.
+           f_equal. assert (b = negb b0) by (apply not_eqb_is_neg; auto).
+           subst. auto.
+Qed.
+
+Theorem free_canon_concat_izo {A: Type} `{Group A} (x y: FreeGroup A) :
+  to_canon (fg_concat x y) = canon_concat (to_canon x) (to_canon y).
+Proof.
+  destruct x as [x |]; auto. cbn. induction x.
+  - cbn. apply free_canon_cons_izo.
+  - cbn. destruct (to_canon' x0) eqn:c.
+    + exfalso. apply (to_canon'_not_nil x0). auto.
+    + destruct p. assert (hd_eq : fg_hd' x0 = (b, a)).
+      { apply some_eq. rewrite free_canon_hd'_izo. cbn. rewrite c. auto. }
+      rewrite hd_eq. cbn in *. rewrite <- IHx. apply free_canon_cons_izo.
+  - cbn. destruct (to_canon' x) eqn:c.
+    + exfalso. apply (to_canon'_not_nil x). auto.
+    + destruct p. assert (hd_eq : fg_hd' x = (b, a0)).
+      { apply some_eq. rewrite free_canon_hd'_izo. cbn. rewrite c. auto. }
+      rewrite hd_eq. cbn in *. rewrite <- IHx. apply free_canon_cons_izo.
+Qed.
+
+Fixpoint canon_apinv {A: Type} `{Group A} (x y: CanonFreeGroup A) :=
+  match x with
+  | [] => y
+  | (b, v) :: x' => canon_apinv x' (cons (negb b, v) y)
+  end.
+
+Definition canon_inv {A: Type} `{Group A} (x: CanonFreeGroup A) := canon_apinv x [].
+
+Fixpoint canon_append {A: Type} `{Group A} (b: bool) (v: A) (x: CanonFreeGroup A) :=
+  match x with
+  | [] => [(b, v)]
+  | [(b', v')] => if negb (eqf v v') || eqb b b'
+                     then [(b', v'); (b, v)]
+                     else []
+  | h :: x' => h :: (canon_append b v x')
+  end.
+
+Theorem group_inv_inv {A: Type} `{Group A} (x: A) : inv (inv x) = x.
+Proof.
+  rewrite <- (right_id (inv (inv x))), <- (left_inv x), <- (op_assoc), left_inv, left_id.
+  auto.
+Qed.
+
+Theorem cons_append_comm {A: Type} `{Group A} (b b': bool) (v v': A) (x: CanonFreeGroup A) :
+  canon_cons b v (canon_append b' v' x) = canon_append b' v' (canon_cons b v x).
+Proof.
+  admit.
+Admitted.
+
+Theorem canon_concat_append {A: Type} `{Group A} (b: bool) (v: A) (x y: CanonFreeGroup A) :
+  canon_concat x (canon_append b v y) = canon_append b v (canon_concat x y).
+Proof.
+  induction x; auto. cbn. destruct a. rewrite IHx. apply cons_append_comm.
+Qed.
+
+Lemma appinv_list_remaining {A: Type} `{Group A} (x y: CanonFreeGroup A) :
+  canon_concat x (canon_apinv x y) = y.
+Proof.
+  revert y. induction x; auto. intros y. cbn. destruct a. rewrite IHx.
+  cbn. rewrite eqf_refl, eqb_negb2. cbn. auto.
+Qed.
+
+Theorem canon_right_inv {A: Type} `{Group A} (x : CanonFreeGroup A) : 
+  canon_concat x (canon_inv x) = [].
+Proof.
+  induction x; auto. cbn. destruct a. rewrite appinv_list_remaining.
+  cbn. rewrite eqf_refl, eqb_negb2. cbn. auto.
+Qed.
+
+Lemma cannon_inv_append {A: Type} `{Group A} (b: bool) (v: A) (x : CanonFreeGroup A) : 
+  canon_inv (x ++ [(b, v)]) = (negb b, v) :: canon_inv x.
+Proof.
+  admit.
+Admitted.
 
 
+Theorem canon_left_inv {A: Type} `{Group A} (x : CanonFreeGroup A) : 
+  canon_concat (canon_inv x) x = [].
+Proof.
+  induction x using rev_ind; auto. destruct x. rewrite cannon_inv_append. cbn.
 
 
 
